src/Assembly/Syntax.v
@@ -207,9 +207,14 @@ Inductive OpCode :=
 | xchg
 | xor
 (* Vectorized opcodes *)
-| vaddps
 | vpaddq    (* Vector packed add quadword integers *)
 | vmovq     (* Vector move quadword *)
+| vpsubq
+| vpandq
+| vporq
+| vpxorq
+| vpaddd
+| vpsubd
 .
 
 Derive OpCode_Listable SuchThat (@FinitelyListable OpCode OpCode_Listable) As OpCode_FinitelyListable.
@@ -299,9 +304,14 @@ Definition accesssize_of_declaration (opc : OpCode) : option AccessSize :=
   | test
   | xchg
   | xor
-  | vaddps
   | vpaddq
   | vmovq
+	| vpsubq
+  | vpandq
+  | vporq
+  | vpxorq
+  | vpaddd
+  | vpsubd
     => None
   end.
 
